L4YAML.lean
@@ -25,6 +25,7 @@ import L4YAML.Proofs.Output.EmitterScannability.WellBracketed
 import L4YAML.Proofs.Output.EmitterScannability.NonemptyStructure
 import L4YAML.Proofs.Output.EmitterScannability
 import L4YAML.Proofs.Output.EmitterScannability.Block
+import L4YAML.Proofs.Output.EmitterScannability.BlockProducers
 import L4YAML.Proofs.Output.IndexedEmitterScannability
 import L4YAML.Proofs.EndToEndCorrectness
 import L4YAML.Proofs.Errors.ErrorProperties
